coq/JsSyntax.v
@@ -391,8 +391,10 @@ Inductive builtin_default_value :=
 
 Inductive builtin_define_own_prop :=
   | builtin_define_own_prop_default
+  (* ARRAYS *)
+  | builtin_define_own_prop_array
   | builtin_define_own_prop_args_obj.
-  (* LATER: string and array *)
+  (* LATER: string *)
 
 
 (**************************************************************)
